<section>  <title> Basic Differentiation</title>
<p></p>
<exercises>
  <title></title>

  <exercisegroup cols="3">
    <title>
      Constant Functions:
    </title>
    <introduction>
      <p>
        Compute <m>\dx{y}</m> for each of the following:
      </p>
    </introduction>
    <exercise>
      <statement>
        <p><m>y=1</m></p>
      </statement>
      <answer>
        <p>
          <m>\dx{y}=0</m>
        </p>
      </answer>
    </exercise>
    <exercise>
      <statement>
        <p>
          <m>
            y=\pi
          </m>
        </p>
      </statement>
      <answer>
        <p>
          <m>\dx{y}=0</m>
        </p>
      </answer>
    </exercise>
    <exercise>
      <statement>
        <p>
          <m>
            y=\pi^3
          </m>
        </p>
      </statement>
      <answer>
        <p>
          <m>\dx{y}=0</m>
        </p>
      </answer>
    </exercise>
    <exercise>
      <statement>
        <p>
          <m>
            y=\dfrac{\sqrt{2}}{\pi}
          </m>
        </p>
      </statement>
      <answer>
        <p>
          <m>\dx{y}=0</m>
        </p>
      </answer>
    </exercise>
    <exercise>
      <statement>
        <p>
          <m>
            y=\sqrt{2}\pi
          </m>
        </p>
      </statement>
      <answer>
        <p>
          <m>\dx{y}=0</m>
        </p>
      </answer>
    </exercise>
    <exercise>
      <statement>
        <p>
          <m>
            y=\dfrac{\pi^{3/2}}{1-\pi}
          </m>
        </p>
      </statement>
      <answer>
        <p>
          <m>\dx{y}=0</m>
        </p>
      </answer>
    </exercise>
    <exercise>
      <statement>
        <p>
          <m>
            y=2,000,000,000
          </m>
        </p>
      </statement>
      <answer>
        <p>
          <m>\dx{y}=0</m>
        </p>
      </answer>
    </exercise>
  </exercisegroup>

  <exercise>
    <statement>
      <p>
        If
        <m>
          y=a^3
        </m>
        is <m>\dx{y}=0</m> or is <m>\dx{y}=3a^2\dx{a}</m>?
      </p>
    </statement>
  </exercise>

  <exercisegroup cols="3"> 
    <title>
      Linear Functions:
    </title>
    <introduction>
      <p>
        Compute <m>\dx{y}</m> for each of the following:
      </p>
    </introduction>
    <exercise>
      <statement>
        <p>
          <m> y=x</m>
        </p>
      </statement>
      <answer>
        <p>
          <m>\dx{y}=\dx{x}</m>
        </p>
      </answer>
    </exercise>
    <exercise>
      <statement>
        <p>
          <m> y=2x</m>
        </p>
      </statement>
      <answer>
        <p>
          <m>\dx{y}=2\dx{x}</m>
        </p>
      </answer>
    </exercise>
    <exercise>
      <statement>
        <p>
          <m> y=20x</m>
        </p>
      </statement>
      <answer>
        <p>
          <m>\dx{y}=20\dx{x}</m>
        </p>
      </answer>
    </exercise>
    <exercise>
      <statement>
        <p>
          <m> y=0.0002x</m>
        </p>
      </statement>
      <answer>
        <p>
          <m>\dx{y}=0.0002\dx{x}</m>
        </p>
      </answer>
    </exercise>
    <exercise>
      <statement>
        <p>
          <m> y=\pi x</m>
        </p>
      </statement>
      <answer>
        <p>
          <m>\dx{y}=\pi \dx{x}</m>
        </p>
      </answer>
    </exercise>
    <exercise>
      <statement>
        <p>
          <m> y=\sqrt{2}x</m>
        </p>
      </statement>
      <answer>
        <p>
          <m>\dx{y}=\sqrt{2}\dx{x}</m>
        </p>
      </answer>
    </exercise>
    <exercise>
      <statement>
        <p>
          <m> y=(\pi+\sqrt{2})x</m>
        </p>
      </statement>
      <answer>
        <p>
          <m>\dx{y}=(\pi+\sqrt{2})\dx{x}</m>
        </p>
      </answer>
    </exercise>
    <exercise>
      <statement>
        <p>
          <m> y=\pi x+\sqrt{2}x</m>
        </p>
      </statement>
      <answer>
        <p>
          <m>\dx{y}=(\pi+\sqrt{2}) \dx{x}</m>
        </p>
      </answer>
    </exercise>
    <exercise>
      <statement>
        <p>
          <m> y=\dfrac{(\pi+\sqrt{2})x}{x}</m>
        </p>
      </statement>
      <answer>
        <p>
          <m>\dx{y}=0</m>
        </p>
      </answer>
    </exercise>
    <exercise>
      <statement>
        <p>
          <m> y=\dfrac{(1-x)x^4}{x^3-x^4}</m>
        </p>
      </statement>
      <answer>
        <p>
          <m>\dx{y}=\dx{x}</m>
        </p>
      </answer>
    </exercise>
  </exercisegroup>

  <exercisegroup cols="3">
    <title>
      Polynomials and Rational Functions:
    </title>
    <introduction>
      <p>
        Compute <m>\dx{y}</m> for each of the following:
      </p>
    </introduction>
    <exercise>
      <statement>
        <p>
          <m> y=x^2</m>
        </p>
      </statement>
      <answer>
        <p>
          <m>\dx{y}=2x\dx{x}</m>
        </p>
      </answer>
    </exercise>
    <exercise>
      <statement>
        <p>
          <m> y=x^3</m>
        </p>
      </statement>
      <answer>
        <p>
          <m>\dx{y}=3x^2\dx{x}</m>
        </p>
      </answer>
    </exercise>
    <exercise>
      <statement>
        <p>
          <m> y=x^2+x^3</m>
        </p>
      </statement>
      <answer>
        <p>
          <m>\dx{y}=\left(2x+3x^2\right)\dx{x}</m>
        </p>
      </answer>
    </exercise>
    <exercise>
      <statement>
        <p>
          <m> y= x^2+x^3 + x^4</m>
        </p>
      </statement>
      <answer>
        <p>
          <m>\dx{y}=\left(2x+3x^2+4x^3\right)\dx{x}</m>
        </p>
      </answer>
    </exercise>
    <exercise>
      <statement>
        <p>
          <m> y= x^2+x^3 + x^4+x^5</m>
        </p>
      </statement>
      <answer>
        <p>
          <m>\dx{y}=\left(5x^4+4x^3+3x^2+2x\right)\dx{x}</m>
        </p>
      </answer>
    </exercise>
    <exercise>
      <statement>
        <p>
          <m> y= x^2-x^3 + x^4-x^5</m>
        </p>
      </statement>
      <answer>
        <p>
          <m>\dx{y}=\left(2x-3x^2+4x^3-5x^4\right)\dx{x}</m>
        </p>
      </answer>
    </exercise>
    <exercise>
      <statement>
        <p>
          <m> y= 2x^2+3x^3</m>
        </p>
      </statement>
      <answer>
        <p>
          <m>\dx{y}=\left(4x+9x^2\right)\dx{x}</m>
        </p>
      </answer>
    </exercise>
    <exercise>
      <statement>
        <p>
          <m> y= 5(2x^2+3x^3)</m>
        </p>
      </statement>
      <answer>
        <p>
          <m>\dx{y}=\left(20x+45x^2\right)\dx{x}</m>
        </p>
      </answer>
    </exercise>
    <exercise>
      <statement>
        <p>
          <m> y= x^{-2}</m>
        </p>
      </statement>
      <answer>
        <p>
          <m>\dx{y}=\dfrac{-2}{x^3}\dx{x}</m>
        </p>
      </answer>
    </exercise>
    <exercise>
      <statement>
        <p>
          <m> y= x^{-3}</m>
        </p>
      </statement>
      <answer>
        <p>
          <m>\dx{y}=\dfrac{-3}{x^4}\dx{x}</m>
        </p>
      </answer>
    </exercise>
    <exercise>
      <statement>
        <p>
          <m> y= x^{-1}</m>
        </p>
      </statement>
      <answer>
        <p>
          <m>\dx{y}=\dfrac{-1}{x^2}\dx{x}</m>
        </p>
      </answer>
    </exercise>
    <exercise>
      <statement>
        <p>
          <m> y= \dfrac1x</m>
        </p>
      </statement>
      <answer>
        <p>
          <m>\dx{y}=-x^{-2}\dx{x}</m>
        </p>
      </answer>
    </exercise>
    <exercise>
      <statement>
        <p>
          <m> y= \dfrac{1}{x^5}</m>
        </p>
      </statement>
      <answer>
        <p>
          <m>\dx{y}=-5x^{-6}\dx{x}</m>
        </p>
      </answer>
    </exercise>
    <exercise>
      <statement>
        <p>
          <m> y= \dfrac1x+\dfrac{1}{x^2}</m>
        </p>
      </statement>
      <answer>
        <p>
          <m>\dx{y}=-x^{-2}-2x^{-3}\dx{x}</m>
        </p>
      </answer>
    </exercise>
    <exercise>
      <statement>
        <p>
          <m> y= \dfrac3x+\dfrac{7}{x^2}</m>
        </p>
      </statement>
      <answer>
        <p>
          <m>\dx{y}=\left(\dfrac{-3}{x^2}-14\dfrac{1}{x^3}\right)\dx{x}</m>
        </p>
      </answer>
    </exercise>
    <exercise>
      <statement>
        <p>
          <m> y= \dfrac3x+\dfrac{-7}{x^2}-\dfrac{5}{x^3}</m>
        </p>
      </statement>
      <answer>
        <p>
          <m>\dx{y}=\left(\dfrac{-3}{x^2}-\dfrac{14}{x^3}+\dfrac{15}{x^4}\right)\dx{x}</m>
        </p>
      </answer>
    </exercise>
    <exercise>
      <statement>
        <p>
          <m> y= x^{3/2}</m>
        </p>
      </statement>
      <answer>

        <p>
          <m>\dx{y}=\frac32 \sqrt{x}\dx{x}</m>
        </p>
      </answer>
    </exercise>
    <exercise>
      <statement>
        <p>
          <m> y= x^{3/2}+x^{-3/2}</m>
        </p>
      </statement>
      <answer>
        <p>
          <m>\dx{y}=\left(\dfrac{3}{2} \sqrt{x}
          -\dfrac{3}{2\sqrt[5]{x}}\right)\dx{x}</m>
        </p>
      </answer>
    </exercise>
    <exercise>
      <statement>
        <p>
          <m> y= \dfrac{3x^5-\dfrac72x^4-\pi x^3}{3x^{1/2}}</m>
        </p>
      </statement>
      <answer>
        <p>
          <m>\dx{y}=\left(\dfrac92
          x^{7/2}-\dfrac{49}{12}x^{5/2}-\frac{5\pi}{6}x^{3/2}\right)\dx{x}</m>
        </p>
      </answer>
    </exercise>
    <exercise>
      <statement>
        <p>
          <m> y= \dfrac{2x^5-7x^{4/3} + x^{-1}- x^{-3}}{x^2}</m>
        </p>
      </statement>
      <answer>
        <p>
          <m>\dx{y}=\left(6x^2+\dfrac{14}{3}x^{-5/3}-\dfrac{3}{x^4}-\dfrac{5}{x^6}\right)\dx{x}</m>
        </p>
      </answer>
    </exercise>
    <exercise>
      <statement>
        <p>
          <m> y= \sqrt{x^3}</m>
        </p>
      </statement>
      <answer>
        <p>
          <m>\dx{y}=\dfrac{3}{2}\sqrt{x}\dx{x}</m>
        </p>
      </answer>
    </exercise>
    <exercise>
      <statement>
        <p>
          <m> y= \sqrt[3]{x^2}</m>
        </p>
      </statement>
      <answer>
        <p>
          <m>\dx{y}=\dfrac{2}{3\sqrt[3]{x}}\dx{x}</m>
        </p>
      </answer>
    </exercise>
    <exercise>
      <statement>
        <p>
          <m> y= 8\sqrt{x^3} - 6\sqrt[3]{x^2}</m>
        </p>
      </statement>
      <answer>
        <p>
          <m>\dx{y}=\left(12\sqrt{x}+\dfrac{4}{\sqrt[3]{x}}\right)\dx{x}</m>
        </p>
      </answer>
    </exercise>

  </exercisegroup>

  <exercisegroup cols="3">
    <title> The Product Rule:</title>
    <introduction>
      <p>
        Compute <m>\dx{y}</m> for each of the
        following:
      </p>
    </introduction>

    <exercise>
      <statement>
        <p>
          <m> 
            y= (2x+3)(3x-2)
          </m>
        </p>
      </statement>
      <answer>
        <p>
          <m>\dx{y}= \left(3(2x+3)+2(3x-2)\right)\dx{x} </m>
        </p>
      </answer>
    </exercise>

    <exercise>
      <statement>
        <p>
          <m> 
            y= (2x^2-1)(x^3+2)
          </m>
        </p>
      </statement>
      <answer>
        <p>
          <m>\dx{y}= \left(3x^2(2x^2-1) + 4x(x^3+2)\right)\dx{x} </m>
        </p>
      </answer>
    </exercise>
    <exercise>
      <statement>
        <p>
          <m> 
            y= (x^2)(x^3+x^2+1)
          </m>
        </p>
      </statement>
      <answer>
        <p>
          <m>\dx{y}=  x^2(3x^2+2x)+2x(x^3+x^2+1)\dx{x}</m>
        </p>
      </answer>
    </exercise>


    <exercise>
      <statement>
        <p>
          <m> 
            y=(x-1)(2x+5)
          </m>
        </p>
      </statement>
      <answer>
        <p>
          <m>\dx{y}= \left(2(x-1)+(2x+5)\left)\dx{x}=\right(4x+3\right)\dx{x}</m>
        </p>
      </answer>
    </exercise>

    <exercise>
      <statement>
        <p>
          <m> 
            y=2x(x^2-x)
          </m>
        </p>
      </statement>
      <answer>
        <p>
          <m>\dx{y}=\left(6x^2-4x\right)\dx{x}</m>
        </p>
      </answer>
    </exercise>



    <exercise>
      <statement>
        <p>
          <m> 
            y= \sqrt{x}\cdot\sqrt[3]{x}
          </m>
        </p>
      </statement>
      <answer>
        <p>
          <m>\displaystyle \dx{y}= \frac{5}{6\sqrt[6]{x}}\dx{x}</m>
        </p>
      </answer>
    </exercise>

  </exercisegroup>

  <exercisegroup cols="3">
    <title> The Quotient Rule:</title>
    <introduction>
      <p>
        Compute <m>\dx{y}</m> for each of the following:
      </p>
    </introduction>
    <exercise>
      <statement>
        <p>
          <m>y=\dfrac{x-1}{x+1}</m>
        </p>
      </statement>
      <answer>
        <p>
          <m> \dx{y}=\dfrac{2}{(x+1)^2}\dx{x}</m>
        </p>
      </answer>
    </exercise>

    <exercise>
      <statement>
        <p>
          <m>y=\dfrac{x^2}{x^2-3x+2}</m>
        </p>
      </statement>
      <answer>
        <p>
          <m> \dx{y} = \dfrac{-x(3x-4)}{(x^2-3x+2)^2}\dx{x}</m>
        </p>
      </answer>
    </exercise>
    <exercise>
      <statement>
        <p>
          <m>y=\dfrac{x^3+x^2}{3x^4-3x^2+2}</m>
        </p>
      </statement>
      <!-- <answer> -->
      <!--   <p> -->
      <!--     <m>y=\dfrac{x^3+x^2-7 x+2}{x-1}</m> -->
      <!--   </p> -->
      <!-- </answer> -->
    </exercise>
    <exercise>
      <statement>
        <p>
          <m>y=\dfrac{\frac{1}{x^2}+\frac1x+2}{x^2+\frac{2}{x^2}}</m>
        </p>
      </statement>
      <answer>
        <p>
          <m> \dx{y}{x} = \dfrac{(x^4+2)(4x+1)-4x^3(2x^2+x+1)}{(x^4+2)^2}\dx{x}</m>
        </p>
      </answer>
    </exercise>
    <exercise>
      <statement>
        <p>
          <m>y=\dfrac{x+1}{x^4+x^3+x^2+x+1}</m>
        </p>
      </statement>
      <answer>
        <p>
          <m> \dx{y} = \dfrac{-(3x^4+6x^2+4x^2+2x)}{(x^4+x^3+x^2+x+1)^2}\dx{x}</m>
        </p>
      </answer>
    </exercise>
    <exercise>
      <statement>
        <p>
          <m>y=\dfrac{x^3+3x^2-x}{x^2+3 x-1}</m>
        </p>
      </statement>
      <answer>
        <p>
          <m> \dx{y} = \dx{x}</m>
        </p>
        <p>
          Strange that the answer is so simple isn't it? I wonder if this is
          really an easy problem in disguise.
        </p>
      </answer>
    </exercise>
    <exercise>
      <statement>
        <p>
          <m>y=\dfrac{x^3-x^2-2x+2}{x-1}</m>
        </p>
      </statement>
      <!-- <hint> -->
      <!--   <p> -->
      <!--     This problem is related to the previous problem. -->
      <!--   </p> -->
      <!-- </hint> -->
      <!-- <answer> -->
      <!--   <p> -->
      <!--     <m> \dx{y} = (2x+2)\dx{x}</m> -->
      <!--   </p> -->
      <!-- </answer> -->
    </exercise>
    <exercise>
      <statement>
        <p>
          <m> \dx{y} =      \dfrac{x^3-2x^2-x+2}{x-2}</m>
        </p>
      </statement>
      <answer>
        <p>
          <m> \dx{y} = 2x\dx{x}</m>
        </p>
      </answer>
    </exercise>
    <exercise>
      <statement>
        <p>
          <m>y=\dfrac{x^3-1}{x^2+x+1}</m>
        </p>
      </statement>
      <!-- <hint> -->
      <!--   <p> -->
      <!--     This problem is related to the previous problem. -->
      <!--   </p> -->
      <!-- </hint> -->
      <!-- <answer> -->
      <!--   <p>  -->
      <!--     <m> \dx{y} = \dx{x}</m> -->
      <!--   </p> -->
      <!-- </answer> -->
    </exercise>
    <!-- <exercise> -->
    <!--   <m>y=\dfrac{5x^8-7x^3+21x-12}{x-1}</m> -->
    <!--   <p> -->
    <!--     <answer> -->
    <!--       <m> \dfdx{y}{x} = </m> -->
    <!--     </answer> -->
    <!--   </p> -->
    <!-- </exercise> -->
    <!-- <exercise> -->
    <!--   <statement> -->
    <!--     <p> -->
    <!--       <m>y=\dfrac{\frac{1}{x-2}-\frac{5}{x+3}}{\frac{1}{x^2+x-6}}</m> -->
    <!--     </p> -->
    <!--   </statement> -->
    <!--   <answer> -->
    <!--     <p> -->
    <!--       <m> \dx{y} = -4\dx{x}</m> -->
    <!--     </p> -->
    <!--   </answer> -->
    <!-- </exercise> -->
    <exercise>
      <statement>
        <p>
          <m>y=\dfrac{x^2(x-1)^2(x+2)^2}{x^3+x^2-2x}</m>
        </p>
      </statement>
      <answer>
        <p>
          <m> \dx{y} = x(x-1) + x(x+2) +(x-1)(x+2)\dx{x}</m>
        </p>
      </answer>
    </exercise>
  </exercisegroup>

  <!-- <exercisegroup cols="6"> -->
  <!--     <exercise> -->
  <!--       <m>  -->
  <!--         y=(x-1)(2x+5) -->
  <!--       </m> -->
  <!--       <answer> -->
  <!--         <m>\dfdx{y}{x}= 2(x-1)+(2x+5)=4x+3</m> -->
  <!--       </answer> -->
  <!--     </exercise> -->

  <!--     <exercise> -->
  <!--       <m>  -->
  <!--         y=2x(x^2-x) -->
  <!--       </m> -->
  <!--       <answer> -->
  <!--         <m>\dfdx{y}{x}=6x^2-4x</m> -->
  <!--       </answer> -->
  <!--     </exercise> -->

  <!--     <exercise> -->
  <!--       <m>  -->
  <!--         y=x\sin(x) -->
  <!--       </m> -->
  <!--       <answer> -->
  <!--         <m>\dfdx{y}{x}= x\cos(x) + \sin(x)</m> -->
  <!--       </answer> -->
  <!--     </exercise> -->

  <!--     <exercise> -->
  <!--       <m>  -->
  <!--         y=x\cos(x) -->
  <!--       </m> -->
  <!--       <answer> -->
  <!--         <m>\dfdx{y}{x}= \cos(x)-x\sin(x)</m> -->
  <!--       </answer> -->
  <!--     </exercise> -->

  <!--     <exercise> -->
  <!--       <m>  -->
  <!--         y=x^2\cos(x) -->
  <!--       </m> -->
  <!--       <answer> -->
  <!--         <m>\dfdx{y}{x}= </m> -->
  <!--       </answer> -->
  <!--     </exercise> -->

  <!--     <exercise> -->
  <!--       <m>  -->
  <!--         y=2\sin(x)\cos(x) -->
  <!--       </m> -->
  <!--       <answer> -->
  <!--         <m>\dfdx{y}{x}= 2\cos(2x)</m> -->
  <!--       </answer> -->
  <!--     </exercise> -->

  <!--     <exercise> -->
  <!--       <m>  -->
  <!--         y=\cos(x)\tan(x) -->
  <!--       </m> -->
  <!--       <answer> -->
  <!--         <m>\dfdx{y}{x}= \cos(x) </m> -->
  <!--       </answer> -->
  <!--     </exercise> -->

  <!--     <exercise> -->
  <!--       <m>  -->
  <!--         y=e^x\sin(x) -->
  <!--       </m> -->
  <!--       <answer> -->
  <!--         <m>\dfdx{y}{x}= e^x(\sin(x)-\cos(x))</m> -->
  <!--       </answer> -->
  <!--     </exercise> -->

  <!--     <exercise> -->
  <!--       <m>  -->
  <!--         y=x^2\sin(x)\cos(x) -->
  <!--       </m> -->
  <!--       <answer> -->
  <!--         <m>\dfdx{y}{x}= </m> -->
  <!--       </answer> -->
  <!--     </exercise> -->

  <!--     <exercise> -->
  <!--       <m>  -->
  <!--         y=x^2\tan(x) -->
  <!--       </m> -->
  <!--       <answer> -->
  <!--         <m>\dfdx{y}{x}= </m> -->
  <!--       </answer> -->
  <!--     </exercise> -->

  <!--     <exercise> -->
  <!--       <m>  -->
  <!--         y=\cos^2(x)-\sin^2(x) -->
  <!--       </m> -->
  <!--       <answer> -->
  <!--         <m>\dfdx{y}{x}= -2\sin(2x)</m> -->
  <!--       </answer> -->
  <!--     </exercise> -->

  <!--     <exercise> -->
  <!--       <m>  -->
  <!--         y=\cos^2(x)+\sin^2(x) -->
  <!--       </m> -->
  <!--       <answer> -->
  <!--         <m>\dfdx{y}{x}= 0</m> -->
  <!--       </answer> -->
  <!--     </exercise> -->

  <!-- <exercise> -->
  <!-- <m>  -->
  <!-- y= \sqrt{x}\cdot\sqrt[3]{x-1} -->
  <!-- </m> -->
  <!-- <answer> -->
  <!-- <m>\dfdx{y}{x}= \frac{5x-3}{6(x-1)^{2/3}x^{1/2}}</m> -->
  <!-- </answer> -->
  <!-- </exercise> -->

  <!-- <exercise> -->
  <!-- <m>  -->
  <!-- y= \sqrt{x}\cdot\sqrt[3]{x} -->
  <!-- </m> -->
  <!-- <answer> -->
  <!-- <m>\displaystyle \dfdx{y}{x}= \frac{5}{6\sqrt[6]{x}}</m> -->
  <!-- </answer> -->
  <!-- </exercise> -->

  <!--   </exercisegroup> -->
  <!-- <exercisegroup cols="6"> -->
  <!--     <exercise> -->
  <!--       <p> -->
  <!--         <m>y = xe^x</m> -->
  <!--       </p> -->
  <!--       <answer> -->
  <!--         <p> -->
  <!--           <m>\dfdx{y}{x}=e^x(x+1)</m> -->
  <!--         </p> -->
  <!--       </answer> -->
  <!--     </exercise> -->
  <!--     <exercise> -->
  <!--       <p> -->
  <!--         <m>y = x^2e^x</m> -->
  <!--       </p> -->
  <!--       <answer> -->
  <!--         <p> -->
  <!--           <m>\dfdx{y}{x}=e^x(x^2+2x)</m> -->
  <!--         </p> -->
  <!--       </answer> -->
  <!--     </exercise> -->
  <!--     <exercise> -->
  <!--       <p> -->
  <!--         <m>y = x^3e^x</m> -->
  <!--       </p> -->
  <!--       <answer> -->
  <!--         <p> -->
  <!--           <m>\dfdx{y}{x}=e^x(x^3+3x^2)</m> -->
  <!--         </p> -->
  <!--       </answer> -->
  <!--     </exercise> -->
  <!--     <exercise> -->
  <!--       <p> -->
  <!--         <m>y = x^4e^x</m> -->
  <!--       </p> -->
  <!--       <answer> -->
  <!--         <p> -->
  <!--           <m>\dfdx{y}{x}=e^x(x^4+4x^3)</m> -->
  <!--         </p> -->
  <!--       </answer> -->
  <!--     </exercise> -->
  <!--     <exercise> -->
  <!--       <p> -->
  <!--         <m>y = x^ne^x</m> -->
  <!--       </p> -->
  <!--     </exercise> -->
  <!-- </exercisegroup> -->
  <!-- <exercisegroup cols="6"> -->
  <!--     <exercise> -->
  <!--       <p> -->
  <!--         <m>y = xe^{-x}</m> -->
  <!--       </p> -->
  <!--       <answer> -->
  <!--         <p> -->
  <!--           <m>\dfdx{y}{x}=-e^x(x-1)</m> -->
  <!--         </p> -->
  <!--       </answer> -->
  <!--     </exercise> -->
  <!--     <exercise> -->
  <!--       <p> -->
  <!--         <m>y = x^2e^{-x}</m> -->
  <!--       </p> -->
  <!--       <answer> -->
  <!--         <p> -->
  <!--           <m>\dfdx{y}{x}=-e^x(x^2-2x)</m> -->
  <!--         </p> -->
  <!--       </answer> -->
  <!--     </exercise> -->
  <!--     <exercise> -->
  <!--       <p> -->
  <!--         <m>y = x^3e^{-x}</m> -->
  <!--       </p> -->
  <!--       <answer> -->
  <!--         <p> -->
  <!--           <m>\dfdx{y}{x}=-e^x(x^3-3x^2)</m> -->
  <!--         </p> -->
  <!--       </answer> -->
  <!--     </exercise> -->
  <!--     <exercise> -->
  <!--       <p> -->
  <!--         <m>y = x^4e^{-x}</m> -->
  <!--       </p> -->
  <!--       <answer> -->
  <!--         <p> -->
  <!--           <m>\dfdx{y}{x}=-e^x(x^4-4x^3)</m> -->
  <!--         </p> -->
  <!--       </answer> -->
  <!--     </exercise> -->
  <!--     <exercise> -->
  <!--       <p> -->
  <!--         <m>y = x^ne^{-x}</m> -->
  <!--       </p> -->
  <!--     </exercise> -->
  <!-- </exercisegroup> -->


<exercisegroup cols="3"><title>Mixed Problems</title>
  <introduction>
    <p>
      Compute <m>\dx{y}</m> in terms of the other variables and
      differentials. Use any method you know:
    </p>
  </introduction>
  <exercise>
    <statement>
      <p>
        <m> y=3x-2z</m>
      </p>
    </statement>
    <answer>
      <p>
        <m>\dx{y}=3\dx{x}-2\dx{z}</m>
      </p>
    </answer>
  </exercise>
  <exercise>
    <statement>
      <p>
        <m> y=4.9x^2+15x+6</m>
      </p>
    </statement>
    <answer>
      <p>
        <m>\dx{y}= 9.8x\dx{x}+15\dx{x}</m>
      </p>
    </answer>
  </exercise>
  <exercise>
    <statement>
      <p>
        <m> y=3.14</m>
      </p>
    </statement>
    <answer>
      <p>
        <m>\dx{y}= 0</m>
      </p>
    </answer>
  </exercise>
  <exercise>
    <statement>
      <p>
        <m> y=3.1416</m>
      </p>
    </statement>
    <answer>
      <p>
        <m>\dx{y}= 0</m>
      </p>
    </answer>
  </exercise>
  <exercise>
    <statement>
      <p>
        <m> y=\pi</m>
      </p>
    </statement>
    <answer>
      <p>
        <m>\dx{y}= 0</m>
      </p>
    </answer>
  </exercise>
    <exercise>
      <statement>
        <p>
          <m> 
            y= \sqrt{x}\cdot\sqrt[3]{x-1}
          </m>
        </p>
      </statement>
      <answer>
        <p>
          <m>\dx{y}= \frac{5x-3}{6(x-1)^{2/3}x^{1/2}}\dx{x}</m>
        </p>
      </answer>
    </exercise>

  <exercise>
    <statement>
      <p>
        <m> y=x^2-2x</m>
      </p>
    </statement>
    <answer>
      <p>
        <m>\dx{y}= 2x\dx{x}-2\dx{x}</m>
      </p>
    </answer>
  </exercise>
  <exercise>
    <statement>
      <p>
        <m> y=\dfrac{x^2-2x}{x}</m>
      </p>
    </statement>
    <answer>
      <p>
        <m>\dx{y}= \dx{x}</m>
      </p>
    </answer>
  </exercise>
  <exercise>
    <statement>
      <p>
        <m> y=3(x^3-4x+2)</m>
      </p>
    </statement>
    <answer>
      <p>
        <m>\dx{y}= 9x^2 \dx{x} -12 \dx{x}  </m>
      </p>
    </answer>
  </exercise>
  <exercise>
    <statement>
      <p>
        <m> y=x^2-\sqrt{x}</m>
      </p>
    </statement>
    <answer>
      <p>
        <m>\dx{y}= \left(2x-\dfrac{1}{2\sqrt{x}}\right)\dx{x} </m>
      </p>
    </answer>
  </exercise>
  <exercise>
    <statement>
      <p>
        <m> y=\dfrac{7x^5-3x^3+x^2}{x}</m>
      </p>
    </statement>
    <answer>
      <p>
        <m>\dx{y}= \left(28x^3-6x^+1\right)\dx{x} </m>
      </p>
    </answer>
  </exercise>
  <exercise>
    <statement>
      <p>
        <m> y=\dfrac{x}{x+1}</m>
      </p>
    </statement>
    <answer>
      <p>
        <m>\dx{y}= \left(\dfrac{1}{(x+1)^2}\right)\dx{x} </m>
      </p>
    </answer>
  </exercise>
  <exercise>
    <statement>
      <p>
        <m>y=xw</m>
      </p>
    </statement>
    <answer>
      <p>
        <m> \dx{y} = x \dx{w} +w \dx{x} </m>
      </p>
    </answer>
  </exercise>
  <exercise>
    <statement>
      <p>
        <m> y=(2x-1)(3x^3+5x^2-6x+7)</m>
      </p>
    </statement>
    <answer>
      <p>
        <m>\dx{y}=
        (2x-1)(9x^2+10x-6)\dx{x}+2(3x^3+5x^2-6x+7)\dx{x}</m>
      </p>
    </answer>

  </exercise>
  <exercise>
    <statement>
      <p>
        <m> y=\left(\sqrt[3]{x}\right)^2-\left(\sqrt{x}\right)^3</m>
      </p>
    </statement>
    <answer>
      <p>
        <m>\dx{y}= \left(\frac23 x^{-1/3}=\frac32x^{1/2}\right)
        \dx{x} </m>
      </p>
    </answer>
  </exercise>
  <exercise>
    <statement>
      <p>
        <m> y=\left(\sqrt[3]{x}\right)^3-\left(\sqrt{x}\right)^2</m>
      </p>
    </statement>
    <answer>
      <p>
        <m>\dx{y}= 0</m>
      </p>
    </answer>
  </exercise>
  <exercise>
    <statement>
      <p>
        <m>
        y=\left(\dfrac{1}{x^2}+\dfrac{1}{x^4}\right)\left(x^2+x^4\right)</m>
      </p>
    </statement>
    <answer>
      <p>
        <m>\dx{y}= \left(2x-2x^{-3}\right)\dx{x} </m>
      </p>
    </answer>
  </exercise>
  <exercise>
    <statement>
      <p>
        <m> y=\left(x^2+x^4\right)\left(x^{-2}+x^{-4}\right)</m>
      </p>
    </statement>
    <answer>
      <p>
        <m>\dx{y}= \left(2x-\dfrac{2}{x^3}\right)\dx{x} </m>
      </p>
    </answer>
  </exercise>
  <!-- <exercise> -->
  <!--   <m> -->
  <!--   y=\inverse{\left(x^2+x^3\right)}\left(x^{-2}+x^{-3}\right)</m> -->
  <!--   <answer> -->
  <!--     <p> -->
  <!--       <m>\dx{y}= </m> -->
  <!--     </p> -->
  <!--   </answer> -->
  <!-- </exercise> -->
  <exercise>
    <statement>
      <p>
        <m> y=x+z+w</m>
      </p>
    </statement>
    <answer>
      <p>
        <m>\dx{y}= \dx{x}+\dx{y}+\dx{w} </m>
      </p>
    </answer>
  </exercise>
  <exercise>
    <statement>
      <p>
        <m> y=\dfrac{x^3-1}{x-3}</m>
      </p>
    </statement>
    <hint>
      <p>
        Can you find a way to use the Product Rule?
      </p>
    </hint>
    <answer>
      <p>
        <m>\dx{y}= \left(\dfrac{2x^3-9x^2+1}{(x-3)^2}\right)\dx{x} </m>
      </p>
    </answer>
  </exercise>
  <exercise>
    <statement>
      <p>
        <m>x=5y^2+2y-3</m>
      </p>
    </statement>
    <hint>
      <p>
        <em>Careful!!</em>
      </p>
    </hint>
    <answer>
      <p>
        <m>\dx{y}= \left(\dfrac{1}{10y+2}\right)\dx{x} </m>
      </p>
    </answer>
  </exercise>
  <exercise>
    <statement>
      <p>
        <m> x^2+y^2=1</m>
      </p>
    </statement>
    <answer>            
      <p>
        <m>\dx{y}= -\left(\dfrac{x}{y}
        \right)\dx{x} </m>
      </p>
    </answer>

  </exercise>
  <exercise>
    <statement>
      <p>
        <m> x^2+y^2+z^2=1</m>
      </p>
    </statement>
    <answer>
      <p>
        <m>\dx{y}= -\dfrac{x \dx{x} + z \dx{z}}{y} </m>
      </p>
    </answer>
  </exercise>
  <exercise>
    <statement>
      <p>
        <m> xy^2=z^3</m>
      </p>
    </statement>
    <answer>            
      <p>
        <m>\dx{y}= \dfrac{3z^2 \dx{z} -y^2 \dx{x}  }{2xy}</m>
      </p>
    </answer>

  </exercise>
  <exercise>
    <statement>
      <p>
        <m>xyz=2</m>
      </p>
    </statement>
    <answer>            
      <p>
        <m>\dx{y}= \dfrac{- xy \dx{z}- yz \dx{x}}{xz}  </m>
      </p>
    </answer>

  </exercise>
  <exercise>
    <statement>
      <p>
        <m> (ct)^2-x^2-y^2-z^2=k^2,</m>
        where <m>c</m> and <m>k</m> are
        constants. <!-- <remark>This equation appears in relativity theory.</remark> -->
      </p>
    </statement>
    <answer>
      <p>
        <m>\dx{y}= \dfrac{x \dx{x} +z \dx{z} -c^2t \dx{t} }{y}</m>
      </p>
    </answer>
  </exercise>
</exercisegroup>
<exercise>
  <statement>
    <p>
      Redo each of the  previous problems, but this time compute
      the ratio: <m>\dfdx{y}{x}</m>.
    </p>
  </statement>
</exercise>

  <exercise><title>Find the Pattern</title>
  <introduction>
    <p>
      Show that <m>\dx{y}</m> is as given for each of the following:
    </p>
  </introduction>
  <task>
    <statement>
      <p>
        <m>y=x+1</m>,
      </p>
      <p>
        <m>\dx{y}=1\dx{x}</m>
      </p>
    </statement>
  </task>
  <task>
    <statement>
      <p>
        <m>y=(x+1)(x+2)</m>,
      </p>
      <p>
        <m>\dx{y}=\left((x+1)+(x+2)\right)\dx{x}</m>
      </p>
    </statement>
  </task>
  <task>
    <statement>
      <p>
        <m>y=(x+1)(x+2)(x+3)</m>
      </p>
      <p>
        <m>\dx{y}=\left((x+1)(x+2) + (x+1)(x+3)+(x+2)(x+3)\right)\dx{x}</m>
      </p>
    </statement>
  </task>
  <task>
    <statement>
      <p>
<m>   y=(x+1)(x+2)(x+3)(x+4)</m>
        <md alignment="alignat">
<mrow>
          \dx{y}=((x+1)(x+2)(x+3) + (x+1)(x+2)(x+4)+{}\amp (x+1)(x+3)(x+4)
</mrow>
<mrow>\amp + (x+2)(x+3)(x+4) )\dx{x}
      </mrow>
        </md>
      </p>
    </statement>
  </task>
  <task>
    <statement>
      <p>
        Now guess the differential of:
        <m>y=(x+1)(x+2)(x+3)(x+4)(x+5)</m>
      </p>
    </statement>
  </task>
  <task>
    <statement>
      <p>
        Now guess what the differential of <m>y=(x+1)(x+2)(x+3)\ \ldots\
        (x+n)</m> will
        be. Can you prove that your guess is correct?
      </p>
    </statement>
  </task>
  <task>
    <statement>
      <p>
        Finally,  what is the differential of
        <m>y=(x+c_1)(x+c_2)(x+c_3)\ldots(x+c_n)</m> if <m>c_1, c_2, c_3,
        \ldots, c_n</m> are assumed to be (unknown) constants?
      </p>
    </statement>
  </task>

  </exercise>



  <exercise>
    <!-- <title> </title> -->
    <introduction>
      <p>
        Show that the differential of each of the following is: <m>
        \dx{y}=\frac{-1}{(x+2)^2}\dx{x}.</m>
      </p>
    </introduction>
    <task>
      <p>
        <m>y=\dfrac{1}{x+2}</m>
      </p>
    </task>
    <task>
      <p>
        <m>y=\dfrac{x+3}{x+2}</m>
      </p>
    </task>
    <task>
      <p>
        <m>y=\dfrac{2x+5}{x+2}</m>
      </p>
    </task>
    <task>
      <p>
        <m>y=\dfrac{-3x-5}{x+2}</m>
      </p>
    </task>
    <task>
      <p>
        Now compute the differential of <m>y=\dfrac{7x+13}{x+2}.</m>
        Why is this one different? 
      </p>
    </task>
  </exercise>


  <exercise>
    <title>Find the Pattern</title>
    <introduction>
      <p>
        Compute <m>\dx{y}</m> for each of the following.
      </p>
    </introduction>

<task>
<statement>
      <p>
        <m>y=\dfrac{1}{x+2}</m>
      </p>
</statement>
<answer>
        <p>
          <m> \dx{y} = \dfrac{-1}{(x+2)^2}\dx{x}</m>
        </p>
      </answer>
</task>

    <task>
<statement>
      <p>
        <m>y=\dfrac{x+1}{x+2}</m>
      </p>
</statement>
<answer>
        <p>
          <m> \dx{y} = \dfrac{1}{(x+2)^2}\dx{x}</m>
        </p>
      </answer>
    </task>

    <task>
<statement>
      <p>
        <m>y=\dfrac{x+1}{x+3}</m>
      </p>
</statement>
<answer>
        <p>
          <m> \dx{y} = \dfrac{2}{(x+3)^2}\dx{x}</m>
        </p>
      </answer>
    </task>

    <task>
<statement>
      <p>
        <m>y=\dfrac{2x+1}{x+3}</m>
      </p>
</statement>
<answer>
        <p>
          <m> \dx{y} = \dfrac{4}{(x+3)^2}\dx{x}</m>
        </p>
      </answer>
    </task>

    <task>
<statement>
      <p>
        <m>y=\dfrac{2x+1}{7x+3}</m>
      </p>
</statement>
<answer>
        <p>
          <m> \dx{y} = \dfrac{-1}{(7x+3)^2}\dx{x}</m>
        </p>
      </answer>
    </task>

    <task>
<statement>
      <p>
        <m>y=\dfrac{2x+5}{7x+3}</m>
      </p>
</statement>
<answer>
        <p>
          <m> \dx{y} = \dfrac{-29}{(7x+3)^2}\dx{x}</m>
        </p>
      </answer>
    </task>
<task>
<statement>
        <p>
          What do you think the  the differential of
          <m>y=\dfrac{ax+b}{cx+d}</m> will be if <m>a, b, c,</m> and
          <m>d</m> are (arbitrary, unknown) constants? Make a conjecture.
        </p>
</statement>
</task>
<task>
<statement>
        <p>
          Check to see if your conjecture works when <m>a=-12, b=-5,
          c=2,</m> and <m>d=-17</m>.  If not, make a new conjecture and try again.
        </p>
</statement>
</task>
  </exercise>

</exercises>
</section>
<!-- Local Variables: -->
<!-- mode: xml -->
<!-- mode: auto-fill t -->
<!-- eval: (load-file "macros.el") -->
<!-- End: -->


