<section>  <title> Making Things "Easier on the Eyes"; The Chain Rule </title>
<p></p>
<exercises><title></title>
<exercisegroup cols="3">
  <introduction>
    <p>
      Find <m>\dx{y}</m> for each of the following. <!-- Check your -->
      <!-- solutions by graphing your computed derivative and the -->
      <!-- one given by your calculator, or Desmos. -->
    </p>
    <!--       <figure> -->
    <!-- <caption> -->
    <!-- </caption> -->
    <!-- <interactive desmos="fkfsrjvn6z" -->
    <!--                      width="150%" aspect="2:1" /> -->
    <!--       </figure> -->
  </introduction>
  <exercise>
    <statement>
      <p>
        <m>y= (2x+3)^6</m>
      </p>
    </statement>
    <answer>
      <p>
        <m>\dx{y}=12(x+3)^5)\dx{x}</m>
      </p>
    </answer>
  </exercise>
  <exercise>
    <statement>
      <p>
        <m>y= (7-3x)^7</m>
      </p>
    </statement>
    <answer>
      <p>
        <m>\dx{y}=-21(7-3x)^6\dx{x}</m>
      </p>
    </answer>
  </exercise>
  <exercise>
    <statement>
      <p>
        <m>y= (7-3x)^{-7}</m>
      </p>
    </statement>
    <answer>
      <p>
        <m>\dx{y}=21(7-3x)^{-8}\dx{x}</m>
      </p>
    </answer>
  </exercise>
  <exercise>
    <statement>
      <p>
        <m>y= \left(\frac{x}{2}+\frac{2}{x}\right)^3</m>
      </p>
    </statement>
    <answer>
      <p>
        <m>\dx{y}=3\left(\frac{x}{2}+\frac{2}{x}\right)^2\left(\frac12-\frac{2}{x^2}\right)\dx{x}</m>
      </p>
    </answer>
  </exercise>
  <exercise>
    <statement>
      <p>
        <m>\displaystyle y=(x^3-1)^2</m>
      </p>
    </statement>
    <answer>
      <p>
        <m> \dx{y} = 6x^5-6x^2\dx{x}</m>
      </p>
    </answer>
  </exercise>
  <exercise>
    <statement>
      <p>
        <m>\displaystyle y=x\sqrt[3]{1+x^2}</m>
      </p>
    </statement>
    <answer>
      <p>
        <m> \dx{y} = \dfrac{\frac53x^2+1}{\sqrt[3]{(1+x^2)^2}}\dx{x}</m>
      </p>
    </answer>
  </exercise>
  <exercise>
    <statement>
      <p>
        <m>\displaystyle y=(2x-3)^4(x^2+x+1)^5</m>
      </p>
    </statement>
    <answer>
      <p>
        <m> \dx{y} =
        (2x-3)^3(x^2+x+1)^4[5(2x-3)(2x+1)+8(x^2+x+1)]\dx{x}</m>
      </p>
    </answer>
  </exercise>
  <exercise>
    <statement>
      <p>
        <m>\displaystyle y=\left(\frac{x^3-1}{x^3+1}\right)^8</m>
      </p>
    </statement>
    <answer>
      <p>
        <m> \dx{y} =\left( \dfrac{48x^2}{(x^3+1)^9}\right)\dx{x}</m>
      </p>
    </answer>
  </exercise>
  <exercise>
<statement>
    <p>
      <m>\displaystyle y=\sqrt{2x+\sqrt{5x-\sqrt{7x}}}</m>
    </p>
</statement>
      <answer>
        <p>
          <m> \dx{y} =
          \frac{1}{2\sqrt{2x+\sqrt{5x-\sqrt{7x}}}}
          \left(
          2+
          \frac{5+\sqrt{\frac{7}{x}}}{2\sqrt{5x-\sqrt{7x}}}
          \right)\dx{x}</m>
        </p>
      </answer>
  </exercise>
  <exercise>
    <statement>
      <p>
        <m>\displaystyle y=[(x^2+3)^3(1-x^3)^2]^5</m>
      </p>
    </statement>
    <answer>
      <p>
        <m> \dx{y} = 5\left[(x^2+3)^3(1-x^3)^2\right]^4\left[6x(1-x^3)(x^2+3)^2(1-3x-x^3)\right]\dx{x}</m>
      </p>
    </answer>
  </exercise>
  <exercise>
    <statement>
      <p>
        <m>\displaystyle y=-\left(\left(-x^2\right)^2-x\right)-\left(\left(-x\right)^3+x\right)^3</m>
      </p>
    </statement>
    <answer>
      <p>
        <m> \dx{y} = \left[2x-1-3(-x^3+x)^2(-3x^2+1)\right]\dx{x}</m>
      </p>
    </answer>
  </exercise>
</exercisegroup>
<exercisegroup cols="2">
    <introduction>
<p>
      Find the pattern.
</p>
    </introduction>
<exercise>
    <task>
      <statement>
        <p>
          <m>\displaystyle y=x^2(x-1)^2</m>
        </p>
      </statement>
      <answer>
        <p>
          <m> \dx{y} = 2x(x-1)(2x-1)\dx{x}</m>
        </p>
      </answer>
    </task>
    <task>
      <statement>
        <p>
          <m>\displaystyle y=x^3(x-1)^3</m>
        </p>
      </statement>
      <answer>
        <p>
          <m> \dx{y} = 3x^2(x-1)^2(2x-1)\dx{x}</m>
        </p>
      </answer>
    </task>
    <task>
      <statement>
        <p>
          <m>\displaystyle y=x^4(x-1)^4</m>
        </p>
      </statement>
      <answer>
        <p>
          <m> \dx{y} = 4x^3(x-1)^3(2x-1)\dx{x}</m>
        </p>
      </answer>
    </task>
    <task>
      <statement>
        <p>
          <m>\displaystyle y=x^a(x-1)^a</m> where <m>a</m> is an unspecified constant.
        </p>
      </statement>
    </task>
  </exercise>

  <exercise>
    <introduction>
<p>
      Find the pattern.
</p>
    </introduction>
    <task>
      <statement>
        <p>
          <m>\displaystyle y=x^2(x-1)^3</m>
        </p>
      </statement>
      <answer>
        <p>
          <m> \dx{y} = x(x-1)^2(5x-2)\dx{x}</m>
        </p>
      </answer>
    </task>
    <task>
      <statement>
        <p>
          <m>\displaystyle y=x^3(x-1)^2</m>
        </p>
      </statement>
      <answer>
        <p>
          <m> \dx{y} = x^2(x-1)(5x-3)\dx{x}</m>
        </p>
      </answer>
    </task>
    <task>
      <statement>
        <p>
          <m>\displaystyle y=x^4(x-1)^7</m>
        </p>
      </statement>
      <answer>
        <p>
          <m> \dx{y} = x^3(x-1)^6(11x-4)\dx{x}</m>
        </p>
      </answer>
    </task>
    <task>
      <statement>
        <p>
          <m>\displaystyle y=x^a(x-1)^b</m> where <m>a</m> and <m>b</m> are unspecified constants.
        </p>
      </statement>
    </task>
  </exercise>

</exercisegroup>
</exercises>
</section>

<!-- Local Variables: -->
<!-- mode: xml -->
<!-- mode: auto-fill t -->
<!-- eval: (load-file "macros.el") -->
<!-- End: -->
 
