<?xml version="1.0" encoding="utf-8"?>
<section>
  <title> Derivatives of Exponential and Logarithm Functions  </title>
  <p></p>
  <exercises><title></title>
<exercisegroup cols="3"><title>Drills:</title>
<introduction>
<p>
For each of the following find <m>\dx{y}</m>:
</p>
</introduction>
<exercise>
      <statement>
        <p>
          <m> 
            y=e^x\sin(x)
          </m>
        </p>
      </statement>
      <answer>
        <p>
          <m>\dx{y}= e^x(\sin(x)+\cos(x))\dx{x}</m>
        </p>
      </answer>
    </exercise>
    <exercise>
      <statement>
        <p>
          <m>y= \dfrac{x}{e^x}</m> 
        </p>
      </statement>
      <answer>
        <p>
          <m> \dx{y}=\frac{1+x}{e^x}\dx{x}</m>
        </p>
      </answer>
    </exercise>
    <!-- <exercise> -->
    <!--   <statement> -->
    <!--     <p> -->
    <!--       <m>y= \dfrac{x}{e^x}</m>, <m>x=1</m> -->
    <!--     </p> -->
    <!--   </statement> -->
    <!--   <answer> -->
    <!--     <p> -->
    <!--       <m>\displaystyle\left. \dfdx{y}{x}\right|_{x=1} = \dfrac2e</m> -->
    <!--     </p> -->
    <!--   </answer> -->
    <!-- </exercise> -->
    <exercise>
      <statement>
        <p>
          <m>y= \dfrac{e^x}{4x^2+3x-5}</m>
        </p>
      </statement>
      <answer>
        <p>
          <!-- <m>\displaystyle\left. \dx{y} = \dfrac{e^x(4x^2+3x-5-(8x+3))}{(4x^2+3x-5)^2}</m> -->
          <m>\displaystyle \dx{y} = \dfrac{e^x(4x^2-5x-8)}{(4x^2+3x-5)^2}</m>
        </p>
      </answer>
    </exercise>
    <!-- <exercise> -->
    <!--   <statement> -->
    <!--     <p> -->
    <!--       <m>y= \dfrac{e^x}{4x^2+3x-5}</m>, <m>x=1</m> -->
    <!--     </p> -->
    <!--   </statement> -->
    <!--   <answer> -->
    <!--     <p> -->
    <!--       <m>\displaystyle\left. \dfdx{y}{x}\right|_{x=1} = \dfrac{-9e}{4}</m> -->
    <!--     </p> -->
    <!--   </answer> -->
    <!-- </exercise> -->
    <exercise>
      <statement>
        <p>
          <m>\displaystyle y=e^{\sin(x)}</m>
        </p>
      </statement>
      <answer>
        <p>
          <m> \dx{y} = e^{\sin(x)}\cos(x)\dx{x}</m>
        </p>
      </answer>
    </exercise>
    <exercise>
      <statement>
        <p>
          <m>\displaystyle y=\sin(e^x)</m>
        </p>
      </statement>
      <answer>
        <p>
          <m> \dx{y} = e^x\cos(e^x)\dx{x}</m>
        </p>
      </answer>
    </exercise>
    <exercise>
      <statement>
        <p>
          <m>\displaystyle y=\cos(e^x)</m>
        </p>
      </statement>
      <answer>
        <p>
          <m> \dx{y} = -e^x\sin(e^x)\dx{x}</m>
        </p>
      </answer>
    </exercise>
<exercise>
      <statement>
        <p>
          <m>\displaystyle y=\frac{e^x}{\ln(x)}</m>
        </p>
      </statement>
      <answer>
        <p>
          <m> \displaystyle\dx{y} = \frac{e^x(x\ln(x)-1)}{x(\ln(x))^2}\dx{x}</m>
        </p>
      </answer>
    </exercise>

<exercise>
      <statement>
        <p>
          <m>\displaystyle y=\frac{\sin(2x)}{\ln(5x)}</m>
        </p>
      </statement>
      <answer>
        <p>
          <m> \displaystyle\dx{y} = \frac{2x\ln(5x)\cos(2x)-\sin(2x)}{x(\ln(5x))^2}\dx{x}</m>
        </p>
      </answer>
    </exercise>

<exercise>
      <statement>
        <p>
          <m>\displaystyle y=e^{(x^2)}</m>
        </p>
      </statement>
      <answer>
        <p>
          <m> \displaystyle\dx{y} = 2xe^{x^2}\dx{x}</m>
        </p>
      </answer>
    </exercise>

<exercise>
      <statement>
        <p>
          <m>\displaystyle y=(e^x)^2</m>
        </p>
      </statement>
      <answer>
        <p>
          <m> \displaystyle\dx{y} = 2(e^x)^2\dx{x}</m>
        </p>
      </answer>
    </exercise>

<exercise>
      <statement>
        <p>
          <m>\displaystyle y=(\ln(x))^2</m>
        </p>
      </statement>
      <answer>
        <p>
          <m> \displaystyle\dx{y} = 2\frac{\ln(x)}{x}\dx{x}</m>
        </p>
      </answer>
    </exercise>

<exercise>
      <statement>
        <p>
          <m>\displaystyle y=\ln(x^2)</m>
        </p>
      </statement>
      <answer>
        <p>
          <m> \displaystyle\dx{y} = \frac{2}{x}\dx{x}</m>
        </p>
      </answer>
    </exercise>


</exercisegroup>
  <exercise>
    <title>Find The Pattern</title>
    <introduction>
      <p> 
        Find, and state, the pattern in the differentials in the next few problems.
      </p>
    </introduction>
    <task>
      <statement>
        <p>
          <m>y = xe^x</m>
        </p>
      </statement>
      <answer>
        <p>
          <m>\dx{y}=e^x(x+1)\dx{x}</m>
        </p>
      </answer>
    </task>
    <task>
      <statement>
        <p>
          <m>y = x^2e^x</m>
        </p>
      </statement>
      <answer>
        <p>
          <m>\dx{y}=e^x(x^2+2x)\dx{x}</m>
        </p>
      </answer>
    </task>
    <task>
      <statement>
        <p>
          <m>y = x^3e^x</m>
        </p>
      </statement>
      <answer>
        <p>
          <m>\dx{y}=e^x(x^3+3x^2)\dx{x}</m>
        </p>
      </answer>
    </task>
    <task>
      <statement>
        <p>
          <m>y = x^4e^x</m>
        </p>
      </statement>
      <answer>
        <p>
          <m>\dx{y}=e^x(x^4+4x^3)\dx{x}</m>
        </p>
      </answer>
    </task>
    <task>
      <statement>
        <p>
          <m>y = x^ne^x</m> where <m>n</m> is any positive integer.
        </p>
      </statement>
      <answer>
        <p>
          <m>\dx{y}=e^x(x^n+nx^{n-1})\dx{x}</m>
        </p>
      </answer>
    </task>
    <task>
      <statement>
        <p>
          <m>y = x^ne^x</m> where <m>n</m> is any negative integer.
        </p>
      </statement>
      <answer>
        <p>
          No.  Find this one on your own. 
        </p>
        <p>
          Be sure to  verify that your answer is correct.
        </p>
      </answer>
    </task>
  </exercise>

  <exercise>
    <title>Find The Pattern</title>
    <introduction>
      <p>
        Find, and state, the pattern for the differentials.
      </p>
    </introduction>
    <task>
      <statement>
        <p>
          <m>y = xe^{-x}</m>
        </p>
      </statement>
      <answer>
        <p>
          <m>\dx{y}=-e^{-x}(x-1)\dx{x}</m>
        </p>
      </answer>
    </task>
    <task>
      <statement>
        <p>
          <m>y = x^2e^{-x}</m>
        </p>
      </statement>
      <answer>
        <p>
          <m>\dx{y}=-e^{-x}(x^2-2x)\dx{x}</m>
        </p>
      </answer>
    </task>
    <task>
      <statement>
        <p>
          <m>y = x^3e^{-x}</m>
        </p>
      </statement>
      <answer>
        <p>
          <m>\dx{y}=-e^{-x}(x^3-3x^2)\dx{x}</m>
        </p>
      </answer>
    </task>
    <task>
      <statement>
        <p>
          <m>y = x^4e^{-x}</m>
        </p>
      </statement>
      <answer>
        <p>
          <m>\dx{y}=-e^{-x}(x^4-4x^3)\dx{x}</m>
        </p>
      </answer>
    </task>
    <task>
      <statement>
        <p>
          <m>y = x^ne^{-x}</m> where <m>n</m> is any positive integer.
        </p>
      </statement>
      <answer>
        <p>
          <m>\dx{y}=-e^{-x}(x^n-nx^{n-1})\dx{x}</m>
        </p>
      </answer>
    </task>
    <task>
      <statement>
        <p>
          <m>y = x^ne^{-x}</m> where <m>n</m> is any negative integer.
        </p>
      </statement>
    </task>
  </exercise>
  <exercise>
    <introduction>
      <p>      Show that <m>\dfdx{y}{x}</m> is the same for all of the
      following.
      </p>
    </introduction>
    <task>
      <p>
        <m>y=\ln(2x)</m>
      </p>
    </task>
    <task>
      <p>
        <m>y=\ln(3x)</m>
      </p>
    </task>
    <task>
      <p>
        <m>y=\ln(4x)</m>
      </p>
    </task>
    <task>
      <p>
        <m>y=\ln(nx)</m>
      </p>
    </task>
  </exercise>

  <exercise>
    <title>Find the Pattern</title>
    <introduction>
      <p>
        Find  <m>\dfdx{y}{x}</m> for each of the following:
      </p>
    </introduction>
    <task>
      <p>
        <m>y=\ln(x^2)</m>
      </p>
    </task>
    <task>
      <p>
        <m>y=\ln(x^3)</m>
      </p>
    </task>
    <task>
      <p>
        <m>y=\ln(x^4)</m>
      </p>
    </task>
    <task>
      <p>
        <m>y=\ln(x^n)</m>
      </p>
    </task>
  </exercise>

  <exercisegroup cols="3">
    <introduction>
      <p>
        Compute the derivative of each of the following.
      </p>
    </introduction>


    <exercise>
      <statement>
        <p>
          <m>y=\ln(3x)+x</m>
        </p>
      </statement>
      <solution>
        <p>
          <m> \dfdx{y}{x} = \dfrac1x +1</m>  
        </p>
      </solution>
    </exercise>
    <exercise>
      <statement>
        <p>
          <m>y=\frac{1}{\ln(3x)}</m>
        </p>
      </statement>
      <solution>
        <p>
          <m>\dfdx{y}{x} = \dfrac{-1}{x[\ln(3x)]^2}</m>
        </p>
      </solution>
    </exercise>
    <exercise>
      <statement>
        <p>
          <m>y=\frac{1}{\ln(\ln(\ln(x)))}</m>
        </p>
      </statement>
      <solution>
        <p>
          <m>\dfdx{y}{x} = \dfrac{1}{\ln(\ln(x))}\cdot\dfrac{1}{\ln(x)}\cdot\dfrac1x</m>
        </p>
      </solution>
    </exercise>
    <exercise>
      <statement>
        <p>
          <m>y=\sqrt{\ln\left(\sqrt{x}\right)}</m>
        </p>
      </statement>
      <solution>
        <p>
          <m>\dfdx{y}{x} = \dfrac{1}{2\sqrt{2}x\ln(\sqrt{x})}</m>
        </p>
      </solution>
    </exercise>
    <exercise>
      <statement>
        <p>
          <m>y=\ln(\sec(x))</m>
        </p>
      </statement>
      <solution>
        <p>
          <m>\dfdx{y}{x} = \tan(x)</m>
        </p>
      </solution>
    </exercise>
    <exercise>
      <statement>
        <p>
          <m>y=\ln(\sec(x)+\tan(x))</m>
        </p>
      </statement>
      <solution>
        <p>
          <m>\dfdx{y}{x} = \sec(x)</m>
        </p>
      </solution>
    </exercise>
<exercise>
        <p>
          <m>y= x\inverse\sec(x) - \ln(x+\sqrt{x^2-1}</m>
        </p>
<answer>
<p>
          <m>\displaystyle\dfdx{y}{x}=\inverse\sec(x)</m>
        </p>
</answer>
</exercise>

<exercise>
        <p>
          <m>y= x\inverse\tan\left(\frac{x}{2}\right)-\ln\left(x^2+4\right)</m>
        </p>
<answer>
<p>
          <m>\displaystyle\dfdx{y}{x}=\inverse\tan(x)</m>
        </p>
</answer>
</exercise>

  </exercisegroup>


  <exercisegroup cols="2">
    <introduction>
      <p>
        Compute the derivative of each of the following pairs of
        functions.
      </p>
    </introduction>
    <exercise>
      <statement>
        <p>
          <md alignment="alignat">
            <mrow> y=\amp\left[x(x+1)\right]^7</mrow>
            <mrow>z=\amp\ln{\left[x(x+1)\right]^7}</mrow>
          </md>
        </p>
      </statement>
      <solution>
        <p>
          <md alignment="alignat">
            <mrow> \dfdx{y}{x} =\amp
            \left[x(x+1)\right]^7\left[\dfrac7x+\dfrac{7}{x+1}\right]</mrow>
            <mrow>\dfdx{z}{x} =\amp \dfrac7x+\dfrac{7}{x+1}</mrow>
          </md>
        </p>
      </solution>
    </exercise>
    <exercise>
      <statement>
        <p>          <md alignment="alignat">
          <mrow>y=\amp\sqrt{x(x+1)}</mrow>
          <mrow>z=\amp\ln\left(\sqrt{x(x+1)}\right)</mrow>
        </md>
        </p>
      </statement>
      <solution>
        <p>
          <md alignment="alignat">
            <mrow>\dfdx{y}{x} =\amp  \left[\sqrt{x(x+1)}\right]\left[\dfrac{1}{2x}+\dfrac{1}{2(x+1)}\right]</mrow>
            <mrow>\dfdx{z}{x} =\amp \dfrac{1}{2x}+\dfrac{1}{2(x+1)} </mrow>
          </md>
        </p>
      </solution>
    </exercise>
    <exercise>
      <statement>
        <p>          
          <md alignment="alignat">
          <mrow>y=\amp x(x-1)(x-2)</mrow>
          <mrow>z=\amp \ln\left(x(x-1)(x-2)\right)</mrow>
        </md>
        </p>
      </statement>
      <solution>
        <p>
          <md alignment="alignat">
            <mrow>\dfdx{y}{x} =\amp 
            \left[x(x-1)(x-2)\right]\left[\dfrac1x+\dfrac{1}{x-1}+\dfrac{1}{x-2}\right]</mrow>
            <mrow>\dfdx{z}{x} =\amp
            \left(\dfrac1x+\dfrac{1}{x-1}+\dfrac{1}{x-2}\right)</mrow>
          </md>
        </p>
      </solution>
    </exercise>
    <exercise>
      <statement>
        <p>          
          <md alignment="alignat">
          <mrow>y=\amp \frac{1}{x(x-1)(x-2)}</mrow>
          <mrow>z=\amp \ln\left(\frac{1}{x(x-1)(x-2)}\right)</mrow>
        </md>
        </p>
      </statement>
      <solution>
        <p>
          <md alignment="alignat">
            <mrow>\dfdx{y}{x} =\amp 
            -\left[\frac{1}{x(x-1)(x-2)}\right]\left[\dfrac1x+\dfrac{1}{x-1}+\dfrac{1}{x-2}\right]</mrow>
            <mrow>\dfdx{z}{x} =\amp 
            -\left(\dfrac1x+\dfrac{1}{x-1}+\dfrac{1}{x-2}\right)</mrow>
          </md>
        </p>
      </solution>
    </exercise>
    <exercise>
      <statement>
        <p><md alignment="alignat">
          <mrow>y=\amp \ln\left({\frac{x\sqrt{x^2+1}}{(x+1)^{2/3}}}\right)</mrow>
          <mrow>z=\amp \frac{x\sqrt{x^2+1}}{(x+1)^{2/3}}</mrow>
        </md>
        </p>
      </statement>
      <solution>
        <p>
          <md alignment="alignat">
            <mrow>\dfdx{y}{x} =\amp  \dfrac1x+\dfrac{x}{x^2+1}-\dfrac{2}{3(x+1)}</mrow>
            <mrow>\dfdx{z}{x} =\amp \left[\frac{x\sqrt{x^2+1}}{(x+1)^{2/3}}\right]\left[\dfrac1x+\dfrac{x}{x^2+1}-\dfrac{2}{3(x+1)}\right]</mrow>
          </md>
        </p>
      </solution>
    </exercise>
    <exercise>
      <statement>
        <p>
          <md alignment="alignat">
            <mrow>y=\amp \ln\left(\sqrt[3]{\frac{x(x+1)(x-2)}{(x^2+1)(2x+3)}}\right)</mrow>
            <mrow>z=\amp \sqrt[3]{\frac{x(x+1)(x-2)}{(x^2+1)(2x+3)}}</mrow>
          </md>
        </p>
      </statement>
      <solution>
        <p>
          <md alignment="alignat">
            <mrow>\dfdx{y}{x} =\amp
            \dfrac13\left(\dfrac1x+\dfrac{1}{x+1}+\dfrac{1}{x-2} -
            \dfrac{x}{x^2-1}-\dfrac{2}{2x+3}\right)</mrow>
            <mrow>\dfdx{z}{x} =\amp
            \dfrac13\left(\sqrt[3]{\frac{x(x+1)(x-2)}{(x^2+1)(2x+3)}}\right)\left(\dfrac1x+\dfrac{1}{x+1}+\dfrac{1}{x-2}
            -
            \dfrac{x}{x^2-1}-\dfrac{2}{2x+3}\right)</mrow>
          </md>
        </p>
      </solution>
    </exercise>
    <exercise>
      <statement>
        <p>
          <md alignment="alignat">
            <mrow>y=\amp e^{2x}</mrow>
            <mrow>z=\amp 2^x</mrow>
          </md>
        </p>
      </statement>
      <solution>
        <p>
          <md alignment="alignat">
            <mrow>\dfdx{y}{x} =\amp 2e^{2x}</mrow>
            <mrow>\dfdx{z}{x} =\amp \left[\ln(2)\right]\cdot 2^x</mrow>
          </md>
        </p>
      </solution>
    </exercise>
    <exercise>
      <statement>
        <p>
          <md alignment="alignat">
            <mrow>y=\amp \frac{\ln(x)}{2}</mrow>
            <mrow>y=\amp \log_2(x)</mrow>
          </md>
        </p>
      </statement>
      <solution>
        <p>
          <md alignment="alignat">
            <mrow>\dfdx{y}{x} =\amp \dfrac{1}{2x}</mrow>
            <mrow>\dfdx{z}{x} =\amp \dfrac{1}{x\ln(2)}</mrow>
          </md>
        </p>
      </solution>
    </exercise>
  </exercisegroup>

  <figure>
    <caption>
      You can use this Desmos interface to check your answers.
    </caption>
    <interactive desmos="vwkddsnyny" width="150%" aspect="2:1" />
  </figure>

  <exercisegroup cols="2"><title>Tangent Lines</title>
  <introduction>
    <p>
      Find an equation of the line tangent to each function below at the given
      point. If no such line exists explain why not.
    </p>
    <p>
      Check your answers by graphing the function and your tangent
      line on the same set of axes. You can use the Desmos interface
      above, open Desmos in another window, use your calculator, or
      any other graphing software to do this. If the line you found
      isn't tangent to the graph then you made a mistake. Try again
      or ask for help.
    </p>
  </introduction>
  <exercise>
    <statement>
      <p>
        <m>y= \dfrac{x}{e^x}</m>, <m>(0,0)</m>
      </p>
      <!-- <solution> -->
      <!--   <m> y = x</m> -->
      <!-- </solution> -->
    </statement>
  </exercise>
  <exercise>
    <statement>
      <p>
        <m>y= \dfrac{x}{e^x}</m>, <m>\left(1,1/e\right)</m>
      </p>
      <!-- <solution> -->
      <!--   <m> y = 1/e</m> -->
      <!-- </solution> -->
    </statement>
  </exercise>
  <exercise>
    <statement>
      <p>
        <m>y= \dfrac{e^x}{4x^2+3x-5}</m>, <m>\left(0,\dfrac{-1}{5}\right)</m>
      </p>
      <!-- <solution> -->
      <!--   <m> y = \frac{8}{25}x-\frac{1}{5}</m> -->
      <!-- </solution> -->
    </statement>
  </exercise>
  <exercise>
    <statement>
      <p>
        <m>y= \dfrac{e^x}{4x^2+3x-5}</m>, <m>(1,e/2)</m>
      </p>
    </statement>
    <!-- <solution> -->
    <!--   <m> y -\dfrac{e}{2}= -\dfrac{9e}{4}(x-1)</m> -->
    <!-- </solution> -->
  </exercise>
  </exercisegroup>
</exercises>
</section>

<!-- Local Variables: -->
<!-- mode: ptx -->
<!-- mode: auto-fill t -->
<!-- eval: (load-file "macros.el") -->
<!-- End: -->


