<section>  <title> The Quotient Rule </title>
<p></p>
<exercises><title></title>
  <exercisegroup cols="3">
    <introduction>
      <p>
        Compute <m>\dfdx{y}{x}</m> for each of the following:
      </p>
    </introduction>
    <exercise>
      <statement>
        <p>
          <m>y=\dfrac{x-1}{x+1}</m>
        </p>
      </statement>
      <answer>
        <p>
          <m> \dfdx{y}{x}=\dfrac{2}{(x-1)^2}</m>
        </p>
      </answer>
    </exercise>

    <exercise>
      <statement>
        <p>
          <m>y=\dfrac{x^2}{x^2-3x+2}</m>
        </p>
      </statement>
      <answer>
        <p>
          <m> \dfdx{y}{x} = \dfrac{-x(3x-4)}{(x^2-3x+2)^2}</m>
        </p>
      </answer>
    </exercise>
    <exercise>
      <statement>
        <p>
          <m>y=\dfrac{x^3+x^2}{3x^4-3x^2+2}</m>
        </p>
      </statement>
      <answer>
        <p>
          <m>y=\dfrac{x^3+x^2-7 x+2}{x-1}</m>
        </p>
      </answer>
    </exercise>
    <exercise>
      <statement>
        <p>
          <m>y=\dfrac{x^3+2x^2+2 x+2}{x^2+3 x-1}</m>
        </p>
      </statement>
      <answer>
        <p>
          <m> \dfdx{y}{x} = 1</m>
        </p>
        <p>
          Strange that the answer is so simple isn't it? I wonder if this is
          really an easy problem in disguise.
        </p>
      </answer>
    </exercise>
    <exercise>
      <statement>
        <p>
          <m>y=\dfrac{x^3+2x^2+2 x+2}{x-1}</m>
        </p>
      </statement>
      <hint>
        <p>          This problem is related to the previous problem.</p>
      </hint>
      <answer>
        <p>
          <m> \dfdx{y}{x} = 2x+3</m>
        </p>
      </answer>
    </exercise>
    <exercise>
      <statement>
        <p>
          <m> \dfdx{y}{x} =      \dfrac{x^3-x^2-x-2}{x-2}</m>
        </p>
      </statement>
      <answer>
        <p>
          <m> \dfdx{y}{x} = 2x+1</m>
        </p>
      </answer>
    </exercise>
    <exercise>
      <statement>
        <p>
          <m>y=\dfrac{x^3-x^2-x-2}{x^2+x+1}</m>
        </p>
      </statement>
      <hint>
        <p>
          If you figured out the last hint, you can use the same technique to do
          this problem.
        </p>
      </hint>
      <answer>
        <p> 
          <m> \dfdx{y}{x} = 1</m>
        </p>
      </answer>
    </exercise>
    <!-- <exercise> -->
    <!--   <m>y=\dfrac{5x^8-7x^3+21x-12}{x-1}</m> -->
    <!--   <p> -->
    <!--     <answer> -->
    <!--       <m> \dfdx{y}{x} = </m> -->
    <!--     </answer> -->
    <!--   </p> -->
    <!-- </exercise> -->
    <exercise>
      <statement>
        <p>
          <m>y=\dfrac{\frac{1}{x-2}-\frac{5}{x+3}}{\frac{1}{x^2+x^-6}}</m>
        </p>
      </statement>
      <answer>
        <p>
          <m> \dfdx{y}{x} = -4</m>
        </p>
      </answer>
    </exercise>
    <exercise>
      <statement>
        <p>
          <m>y=\dfrac{\frac{1}{x^2}+\frac1x+2}{x^2+\frac{2}{x^2}}</m>
        </p>
      </statement>
      <answer>
        <p>
          <m> \dfdx{y}{x} = \dfrac{(x^4+2)(4x+1)-4x^3(2x^2+x+1)}{(x^4+2)^2}</m>
        </p>
      </answer>
    </exercise>
    <exercise>
      <statement>
        <p>
          <m>y=\dfrac{x+1}{x^4+x^3+x^2+x+1}</m>
        </p>
      </statement>
      <answer>
        <p>
          <m> \dfdx{y}{x} = \dfrac{-(3x^2-2x+1)}{(x^3-x^2+x-1)^2}</m>
        </p>
      </answer>
    </exercise>
    <exercise>
      <statement>
        <p>
          <m>y=\dfrac{x^2(x-1)^2(x+2)^2}{x^3+x^2-2x}</m>
        </p>
      </statement>
      <answer>
        <p>
          <m> \dfdx{y}{x} = x(x-1) + x(x+2) +(x-1)(x+2)</m>
        </p>
      </answer>
    </exercise>
  </exercisegroup>


  <exercise>
    <title> </title>
    <introduction>
      <p>
        Show that the derivative of each of the following is: <m>
        \dfdx{y}{x}=\frac{-1}{(x+2)^2}.</m>
      </p>
    </introduction>
    <task>
      <p>
        <m>y=\dfrac{1}{x+2}</m>
      </p>
    </task>
    <task>
      <p>
        <m>y=\dfrac{x+3}{x+2}</m>
      </p>
    </task>
    <task>
      <p>
        <m>y=\dfrac{2x+5}{x+2}</m>
      </p>
    </task>
    <task>
      <p>
        <m>y=\dfrac{-3x-5}{x+2}</m>
      </p>
    </task>
    <task>
      <p>
        Now compute the derivative of <m>y=\dfrac{7x+13}{x+2}.</m>
        Why is this one different? 
      </p>
    </task>
  </exercise>


  <exercise>
    <title>Find the Pattern</title>
    <introduction>
      <p>
        Compute <m>\dfdx{y}{x}</m> for each of the following.
      </p>
    </introduction>

<task>
<statement>
      <p>
        <m>y=\dfrac{1}{x+2}</m>
      </p>
</statement>
<answer>
        <p>
          <m> \dfdx{y}{x} = \dfrac{-1}{(x+2)^2}</m>
        </p>
      </answer>
</task>

    <task>
<statement>
      <p>
        <m>y=\dfrac{x+1}{x+2}</m>
      </p>
</statement>
<answer>
        <p>
          <m> \dfdx{y}{x} = \dfrac{1}{(x+2)^2}</m>
        </p>
      </answer>
    </task>

    <task>
<statement>
      <p>
        <m>y=\dfrac{x+1}{x+3}</m>
      </p>
</statement>
<answer>
        <p>
          <m> \dfdx{y}{x} = \dfrac{2}{(x+3)^2}</m>
        </p>
      </answer>
    </task>

    <task>
<statement>
      <p>
        <m>y=\dfrac{2x+1}{x+3}</m>
      </p>
</statement>
<answer>
        <p>
          <m> \dfdx{y}{x} = \dfrac{4}{(x+3)^2}</m>
        </p>
      </answer>
    </task>

    <task>
<statement>
      <p>
        <m>y=\dfrac{2x+1}{7x+3}</m>
      </p>
</statement>
<answer>
        <p>
          <m> \dfdx{y}{x} = \dfrac{-1}{(7x+3)^2}</m>
        </p>
      </answer>
    </task>

    <task>
<statement>
      <p>
        <m>y=\dfrac{2x+5}{7x+3}</m>
      </p>
</statement>
<answer>
        <p>
          <m> \dfdx{y}{x} = \dfrac{-29}{(7x+3)^2}</m>
        </p>
      </answer>
    </task>
<task>
<statement>
        <p>
          What do you think the  the derivative of
          <m>y=\dfrac{ax+b}{cx+d}</m> will be if <m>a, b, c,</m> and
          <m>d</m> are (arbitrary, unknown) constants? Make a conjecture.
        </p>
</statement>
</task>
<task>
<statement>
        <p>
          Check to see if your conjecture works when <m>a=-12, b=-5,
          c=2,</m> and <m>d=-17</m>.  If not, try again.
        </p>
</statement>
</task>
  </exercise>


  <!-- <exercise> -->
  <!--   <p> -->
  <!--     Compute <m>\dfdx{y}{x}</m> for each of the following: -->
  <!--   </p> -->
  <!--   <ol cols="2" marker="(a)"> -->
  <!--     <li> -->
  <!--       <m>f(x)=\dfrac{1}{x+1}</m> -->
  <!--     </li> -->
  <!--     <li> -->
  <!--       <m>f(x)=\dfrac{1}{(x+1)(x+2)}</m> -->
  <!--     </li> -->
  <!--     <li> -->
  <!--       <m>f(x)=\dfrac{1}{(x+3)(x+4)}</m> -->
  <!--     </li> -->
  <!--     <li> -->
  <!--       <m>f(x)=\dfrac{1}{(x+5)(x+7)}</m> -->
  <!--     </li> -->
  <!--     <li> -->
  <!--       <m>f(x)=\dfrac{1}{(x+a)(x+b)}</m> -->
  <!--       <p> -->
  <!--         (<m>a</m> and <m>b</m> are constants) -->
  <!--       </p> -->
  <!--     </li> -->
  <!--     <li> -->
  <!--       <m>f(x)=\dfrac{1}{(x+a)(x+b)(x+c)}</m> -->
  <!--       <p> -->
  <!--         (<m>a, b</m> and <m>c</m> are constants) -->
  <!--       </p> -->
  <!--     </li> -->
  <!--   </ol> -->
  <!-- </exercise> -->
</exercises>
</section>
<!-- Local Variables: -->
<!-- mode: xml -->
<!-- mode: auto-fill t -->
<!-- eval: (load-file "macros.el") -->
<!-- End: -->


